Definte {Simple,Boolean}Recognizer in terms of the generic one

src/Parsers/BooleanRecognizerCorrect.v
@@ -1,16 +1,13 @@
+Require Import Coq.Classes.Morphisms.
+Require Import Fiat.Parsers.StringLike.Core.
 Require Import Fiat.Parsers.ContextFreeGrammar.Core.
-Require Import Fiat.Parsers.BooleanRecognizerMin Fiat.Parsers.BooleanRecognizer Fiat.Parsers.BooleanRecognizerExt.
-Require Import Fiat.Parsers.MinimalParse.
 Require Import Fiat.Parsers.BaseTypes Fiat.Parsers.CorrectnessBaseTypes.
-Require Import Fiat.Parsers.BaseTypesLemmas.
-Require Import Fiat.Parsers.Splitters.RDPList Fiat.Parsers.Splitters.BruteForce.
-Require Import Fiat.Parsers.MinimalParseOfParse.
-Require Import Fiat.Parsers.ContextFreeGrammar.Properties Fiat.Parsers.WellFoundedParse.
-Require Import Fiat.Common Fiat.Common.Wf.
-Require Import Fiat.Common.List.ListFacts.
-Require Import Fiat.Parsers.ParserInterface.
-Require Import Fiat.Parsers.ContextFreeGrammar.Valid Fiat.Parsers.ContextFreeGrammar.ValidProperties.
-Local Open Scope string_like_scope.
+Require Import Fiat.Parsers.GenericBaseTypes Fiat.Parsers.GenericCorrectnessBaseTypes.
+Require Import Fiat.Parsers.ContextFreeGrammar.Valid.
+Require Import Fiat.Parsers.GenericRecognizerCorrect.
+Require Import Fiat.Parsers.BooleanRecognizer.
+
+Local Coercion is_true : bool >-> Sortclass.
 
 Section convenience.
   Context {Char} {HSLM : StringLikeMin Char} {HSL : StringLike Char} {HSLP : StringLikeProperties Char} {G : grammar Char}.
@@ -19,65 +16,39 @@ Section convenience.
           {rdata : @parser_removal_dataT' _ G _}
           (gvalid : grammar_valid G).
 
-  Local Ltac invert_bool_of_sum :=
-    progress
-      repeat match goal with
-               | [ H : is_true false |- _ ] => solve [ inversion H ]
-               | [ |- is_true true ] => reflexivity
-               | [ H : context[bool_of_sum _] |- _ ] => revert H
-               | [ |- context[bool_of_sum ?e] ] => case e; simpl
-               | _ => progress intros
-               | [ |- is_true false ] => exfalso
-               | [ H : _ -> False |- False ] => apply H; clear H
-             end.
+  Local Instance gencdata_default_proper {A}
+    : Proper (beq ==> eq ==> eq ==> eq ==> Basics.impl) (fun _ (_ : A) (x y : bool) => y = x).
+  Proof.
+    repeat intro; repeat subst; reflexivity.
+  Qed.
+
+  Local Existing Instance boolean_gendata.
+  Global Program Instance boolean_gencdata : generic_parser_correctness_dataT
+    := { parse_nt_is_correct str nt exp act := act = exp;
+         parse_item_is_correct str it exp act := act = exp;
+         parse_production_is_correct str p exp act := act = exp;
+         parse_productions_is_correct str p exp act := act = exp }.
 
   Definition parse_item_sound
-             (str : String) (it : item Char)
-  : parse_item str it
-    -> parse_of_item G str it.
-  Proof.
-    intro pit.
-    erewrite <- parse_item_eq in pit by eassumption; invert_bool_of_sum.
-    apply parse_of_item__of__minimal_parse_of_item in m.
-    apply m.
-  Defined.
+    : forall str it, parse_item str it -> parse_of_item G str it
+    := parse_item_sound.
 
   Definition parse_item_complete
-             (str : String) (it : item Char)
-             (p : parse_of_item G str it)
-  : parse_item str it.
-  Proof.
-    erewrite <- parse_item_eq by assumption; invert_bool_of_sum.
-    apply minimal_parse_of_item__of__parse_of_item; assumption.
-  Qed.
+    : forall str it, parse_of_item G str it -> parse_item str it
+    := parse_item_complete.
 
   Definition parse_nonterminal_sound
-             (str : String) (nt : String.string)
-  : parse_nonterminal str nt
-    -> parse_of_item G str (NonTerminal nt).
-  Proof.
-    intro pit.
-    erewrite <- parse_nonterminal_eq in pit by eassumption; invert_bool_of_sum.
-    apply parse_of_item_nonterminal__of__minimal_parse_of_nonterminal in m.
-    apply m.
-  Defined.
+    : forall str nt, parse_nonterminal str nt -> parse_of_item G str (NonTerminal nt)
+    := parse_nonterminal_sound.
 
   Definition parse_nonterminal_complete
-             (str : String) (nt : String.string)
-             (p : parse_of_item G str (NonTerminal nt))
-  : parse_nonterminal str nt.
-  Proof.
-    erewrite <- parse_nonterminal_eq by assumption; invert_bool_of_sum.
-    apply minimal_parse_of_nonterminal__of__parse_of_item_nonterminal.
-    assumption.
-  Qed.
+    : forall str nt, parse_of_item G str (NonTerminal nt) -> parse_nonterminal str nt
+    := parse_nonterminal_complete.
 
   Definition parse_of_nonterminal_complete
-             (str : String) (nt : String.string)
-             (H : List.In nt (Valid_nonterminals G))
-             (p : parse_of G str (Lookup G nt))
-  : parse_nonterminal str nt.
-  Proof.
-    apply (parse_nonterminal_complete (ParseNonTerminal _ H p)).
-  Qed.
+    : forall str nt,
+      List.In nt (Valid_nonterminals G)
+      -> parse_of G str (Lookup G nt)
+      -> parse_nonterminal str nt
+    := parse_of_nonterminal_complete.
 End convenience.
