src/Parsers/SimpleRecognizer.v
@@ -1,11 +1,14 @@
 (** * Definition of a simple_parse_of-returning CFG parser-recognizer *)
+(** * Definition of a boolean-returning CFG parser-recognizer *)
 Require Import Coq.Lists.List.
 Require Import Coq.Arith.EqNat.
 Require Import Coq.Arith.Compare_dec Coq.Arith.Wf_nat.
 Require Import Coq.omega.Omega.
 Require Import Fiat.Parsers.ContextFreeGrammar.Core.
 Require Import Fiat.Parsers.BaseTypes.
+Require Import Fiat.Parsers.GenericBaseTypes.
 Require Import Fiat.Parsers.StringLike.Properties.
+Require Import Fiat.Parsers.GenericRecognizer.
 Require Import Fiat.Common Fiat.Common.Wf.
 
 Set Implicit Arguments.
@@ -19,243 +22,104 @@ Section recursive_descent_parser.
   Local Notation simple_parse_of := (@simple_parse_of Char) (only parsing).
   Local Notation simple_parse_of_production := (@simple_parse_of_production Char) (only parsing).
 
-  Section simple.
-    Section parts.
-      Definition parse_item'
-                 (str_matches_nonterminal : nonterminal_carrierT -> option simple_parse_of)
-                 (offset : nat) (len : nat)
-                 (it : item Char)
-      : option simple_parse_of_item
-        := match it with
-             | Terminal P => if EqNat.beq_nat len 1 && char_at_matches offset str P
-                             then Some (SimpleParseTerminal (unsafe_get offset str))
-                             else None
-             | NonTerminal nt => if is_valid_nonterminal initial_nonterminals_data (of_nonterminal nt)
-                                 then option_map
-                                        (SimpleParseNonTerminal nt)
-                                        (str_matches_nonterminal (of_nonterminal nt))
-                                 else None
-           end%bool.
+  Definition option_SimpleParseProductionCons
+    : option simple_parse_of_item
+      -> option simple_parse_of_production
+      -> option simple_parse_of_production
+    := fun pit pits
+       => match pit, pits with
+          | Some pit', Some pits' => Some (SimpleParseProductionCons pit' pits')
+          | None, _ => None
+          | _, None => None
+          end.
 
-      Section production.
-        Context {len0}
-                (parse_nonterminal
-                 : forall (offset : nat) (len : nat),
-                     len <= len0
-                     -> nonterminal_carrierT
-                     -> option simple_parse_of).
+  Definition option_orb {A} (x y : option A) : option A
+    := match x, y with
+       | Some x', _ => Some x'
+       | None, Some y' => Some y'
+       | None, None => None
+       end.
 
-        Definition option_SimpleParseProductionCons
-        : option simple_parse_of_item
-          -> option simple_parse_of_production
-          -> option simple_parse_of_production
-          := fun pit pits
-             => match pit, pits with
-                  | Some pit', Some pits' => Some (SimpleParseProductionCons pit' pits')
-                  | None, _ => None
-                  | _, None => None
-                end.
+  Definition option_simple_parse_of_orb
+             (x : option simple_parse_of_production)
+             (xs : option simple_parse_of)
+    : option simple_parse_of
+    := match x, xs with
+       | Some x', _ => Some (SimpleParseHead x')
+       | None, Some xs' => Some (SimpleParseTail xs')
+       | None, None => None
+       end.
 
-        Definition option_orb {A} (x y : option A) : option A
-          := match x, y with
-               | Some x', _ => Some x'
-               | None, Some y' => Some y'
-               | None, None => None
-             end.
+  Local Instance simple_gendata : generic_parser_dataT Char
+    := { parse_nt_T := option simple_parse_of;
+         parse_item_T := option simple_parse_of_item;
+         parse_production_T := option simple_parse_of_production;
+         parse_productions_T := option simple_parse_of;
+         ret_Terminal_false ch := None;
+         ret_Terminal_true ch := Some (SimpleParseTerminal ch);
+         ret_NonTerminal_false nt := None;
+         ret_NonTerminal_true nt := option_map (SimpleParseNonTerminal nt);
+         ret_production_cons := option_SimpleParseProductionCons;
+         ret_orb_production := option_orb;
+         ret_orb_production_base := None;
+         ret_production_nil_true := Some SimpleParseProductionNil;
+         ret_production_nil_false := None;
+         ret_orb_productions := option_simple_parse_of_orb;
+         ret_orb_productions_base := None;
+         ret_nt b := b;
+         ret_nt_invalid := None }.
 
-        (** To match a [production], we must match all of its items.
-            But we may do so on any particular split. *)
-        Definition parse_production'_for
-                 (splits : production_carrierT -> String -> nat -> nat -> list nat)
-                 (offset : nat)
-                 (len : nat)
-                 (pf : len <= len0)
-                 (prod_idx : production_carrierT)
-        : option simple_parse_of_production.
-        Proof.
-          revert offset len pf.
-          refine
-            (list_rect
-               (fun _ =>
-                  forall (idx : production_carrierT)
-                         (offset : nat)
-                         (len : nat)
-                         (pf : len <= len0),
-                    option simple_parse_of_production)
-               ((** 0-length production, only accept empty *)
-                 fun _ offset len _ => if beq_nat len 0
-                                       then Some SimpleParseProductionNil
-                                       else None)
-               (fun it its parse_production' idx offset len pf
-                => fold_left
-                     option_orb
-                     (map (fun n =>
-                             option_SimpleParseProductionCons
-                               (parse_item'
-                                  (parse_nonterminal offset (len := min n len) _)
-                                  offset
-                                  (min n len)
-                                  it)
-                               (parse_production' (production_tl idx) (offset + n) (len - n) _))
-                          (splits idx str offset len))
-                     None)
-               (to_production prod_idx)
-               prod_idx);
-          clear -pf;
-          abstract (try apply Min.min_case_strong; omega).
-        Defined.
+  Definition parse_item'
+    := Eval cbv [parse_item' parse_nt_T parse_item_T parse_production_T simple_gendata] in
+        parse_item' str.
 
-        Definition parse_production'
-                 (offset : nat)
-                 (len : nat)
-                 (pf : len <= len0)
-                 (prod_idx : production_carrierT)
-        : option simple_parse_of_production
-          := parse_production'_for split_string_for_production offset pf prod_idx.
-      End production.
+  Definition parse_production'_for {len0}
+    := Eval cbv [parse_production'_for parse_nt_T simple_gendata parse_production_T] in
+        parse_production'_for str (len0 := len0).
 
-      Section productions.
-        Context {len0}
-                (parse_nonterminal
-                 : forall (offset : nat)
-                          (len : nat)
-                          (pf : len <= len0),
-                     nonterminal_carrierT -> option simple_parse_of).
+  Definition parse_production' {len0}
+    := Eval cbv [parse_production' parse_nt_T simple_gendata parse_production_T] in
+        parse_production' str (len0 := len0).
 
-        Definition option_simple_parse_of_orb
-                   (x : option simple_parse_of_production)
-                   (xs : option simple_parse_of)
-        : option simple_parse_of
-          := match x, xs with
-               | Some x', _ => Some (SimpleParseHead x')
-               | None, Some xs' => Some (SimpleParseTail xs')
-               | None, None => None
-             end.
+  Definition parse_productions' {len0}
+    := Eval cbv [parse_productions' parse_nt_T simple_gendata parse_production_T] in
+        parse_productions' str (len0 := len0).
 
-        (** To parse as a given list of [production]s, we must parse as one of the [production]s. *)
-        Definition parse_productions'
-                   (offset : nat)
-                   (len : nat)
-                   (pf : len <= len0)
-                   (prods : list production_carrierT)
-        : option simple_parse_of
-          := fold_right option_simple_parse_of_orb
-                        None
-                        (map (parse_production' parse_nonterminal offset pf)
-                             prods).
-      End productions.
+  Definition parse_nonterminal_step {len0 valid_len}
+    := Eval cbv [parse_nonterminal_step parse_nt_T simple_gendata parse_production_T] in
+        parse_nonterminal_step str (len0 := len0) (valid_len := valid_len).
 
+  Definition parse_nonterminal_or_abort
+    : forall (p : nat * nat)
+             (valid : nonterminals_listT)
+             (offset : nat) (len : nat),
+      len <= fst p
+      -> nonterminal_carrierT
+      -> option simple_parse_of
+    := parse_nonterminal_or_abort str.
 
-      Section nonterminals.
-        Section step.
-          Context {len0 valid_len}
-                  (parse_nonterminal
-                   : forall (p : nat * nat),
-                       prod_relation lt lt p (len0, valid_len)
-                       -> forall (valid : nonterminals_listT)
-                                 (offset : nat) (len : nat),
-                            len <= fst p -> nonterminal_carrierT -> option simple_parse_of).
+  Definition parse_nonterminal'
+             (nt : nonterminal_carrierT)
+    : option simple_parse_of
+    := parse_nonterminal' str nt.
 
-          Definition parse_nonterminal_step
-                     (valid : nonterminals_listT)
-                     (offset : nat)
-                     (len : nat)
-                     (pf : len <= len0)
-                     (nt : nonterminal_carrierT)
-          : option simple_parse_of.
-          Proof.
-            refine
-              (option_rect
-                 (fun _ => option simple_parse_of)
-                 (fun parse_nonterminal
-                  => parse_productions'
-                       parse_nonterminal
-                       offset
-                       (len := len)
-                       (sumbool_rect
-                          (fun b => len <= (if b then len else len0))
-                          (fun _ => le_n _)
-                          (fun _ => _)
-                          (lt_dec len len0))
-                       (nonterminal_to_production nt))
-                 None
-                 (sumbool_rect
-                    (fun b => option (forall (offset' : nat) (len' : nat), len' <= (if b then len else len0) -> nonterminal_carrierT -> option simple_parse_of))
-                    (fun _ => (** [str] got smaller, so we reset the valid nonterminals list *)
-                       Some (@parse_nonterminal
-                               (len, nonterminals_length initial_nonterminals_data)
-                               (or_introl _)
-                               initial_nonterminals_data))
-                    (fun _ => (** [str] didn't get smaller, so we cache the fact that we've hit this nonterminal already *)
-                       sumbool_rect
-                         (fun _ => option (forall (offset' : nat) (len' : nat), len' <= len0 -> nonterminal_carrierT -> option simple_parse_of))
-                         (fun is_valid => (** It was valid, so we can remove it *)
-                            Some (@parse_nonterminal
-                                    (len0, pred valid_len)
-                                    (or_intror (conj eq_refl _))
-                                    (remove_nonterminal valid nt)))
+  Definition parse_nonterminal
+             (nt : String.string)
+    : option simple_parse_of
+    := parse_nonterminal str nt.
 
-                         (fun _ => (** oops, we already saw this nonterminal in the past.  ABORT! *)
-                            None)
-                         (Sumbool.sumbool_of_bool (negb (EqNat.beq_nat valid_len 0) && is_valid_nonterminal valid nt)))
-                    (lt_dec len len0)));
-            first [ assumption
-                  | simpl;
-                    generalize (proj1 (proj1 (Bool.andb_true_iff _ _) is_valid));
-                    clear; intro;
-                    abstract (
-                        destruct valid_len; try apply Lt.lt_n_Sn; [];
-                        exfalso; simpl in *; congruence
-                  ) ].
-          Defined.
-        End step.
+  Definition parse_item
+             (it : item Char)
+    : option simple_parse_of_item
+    := parse_item str it.
 
-        Section wf.
-          (** TODO: add comment explaining signature *)
-          Definition parse_nonterminal_or_abort
-          : forall (p : nat * nat)
-                   (valid : nonterminals_listT)
-                   (offset : nat) (len : nat),
-              len <= fst p
-              -> nonterminal_carrierT
-              -> option simple_parse_of
-            := @Fix
-                 (nat * nat)
-                 _
-                 (well_founded_prod_relation lt_wf lt_wf)
-                 _
-                 (fun sl => @parse_nonterminal_step (fst sl) (snd sl)).
+  Definition parse_production
+             (pat : production_carrierT)
+    : option simple_parse_of_production
+    := parse_production str pat.
 
-          Definition parse_nonterminal'
-                     (nt : nonterminal_carrierT)
-          : option simple_parse_of
-            := @parse_nonterminal_or_abort
-                 (length str, nonterminals_length initial_nonterminals_data)
-                 initial_nonterminals_data
-                 0 (length str)
-                 (le_n _) nt.
-
-          Definition parse_nonterminal
-                     (nt : String.string)
-          : option simple_parse_of
-            := parse_nonterminal' (of_nonterminal nt).
-        End wf.
-      End nonterminals.
-
-      Definition parse_item
-                 (it : item Char)
-      : option simple_parse_of_item
-        := parse_item' parse_nonterminal' 0 (length str) it.
-
-      Definition parse_production
-                 (pat : production_carrierT)
-      : option simple_parse_of_production
-        := parse_production' (parse_nonterminal_or_abort (length str, nonterminals_length initial_nonterminals_data) initial_nonterminals_data) 0 (reflexivity _) pat.
-
-      Definition parse_productions
-                 (pats : list production_carrierT)
-      : option simple_parse_of
-        := parse_productions' (parse_nonterminal_or_abort (length str, nonterminals_length initial_nonterminals_data) initial_nonterminals_data) 0 (reflexivity _) pats.
-    End parts.
-  End simple.
+  Definition parse_productions
+             (pats : list production_carrierT)
+    : option simple_parse_of
+    := parse_productions str pats.
 End recursive_descent_parser.
